Fixing wcc

dataplane/Timely_Dataflow_Op.thy
@@ -191,7 +191,7 @@ definition "is_busy sg op = (case get_nid op of None \<Rightarrow> True
           frontier (c_imp (pt_tr sg) (Loc nid (Src p))) \<noteq> {}\<^sub>A))"
 
 corec opt_dataflow_op where
-  "opt_dataflow_op sg op = Choice (cimage (\<lambda> op. case op of
+  "opt_dataflow_op (sg :: (_, _, (nat, nat) myprod, _) subgraph_scheme) op = Choice (cimage (\<lambda> op. case op of
      Read (Inl nid) f \<Rightarrow> (case propagate_all (summ sg) (pt_tr sg) of
          Some conf' \<Rightarrow> let sg' = sg\<lparr> pt_tr := conf', upfro := (upfro sg)(nid := False) \<rparr> in
          let imp_fron = (\<lambda> p. c_imp (pt_tr sg') (Loc nid (Trg p))) in Silent (opt_dataflow_op sg' (f (Inl (Inr (frontier o imp_fron)))))
@@ -201,9 +201,41 @@ corec opt_dataflow_op where
    | Silent op' \<Rightarrow> Silent (opt_dataflow_op sg op')
    | Write op' (Inl nid) (Inl (Inl st)) \<Rightarrow> Silent (opt_dataflow_op (sg\<lparr> upfro := (\<lambda> _. True), pt_tr := change_multiplicities (summ sg) (extract_progress nid (nxt sg) st) (pt_tr sg) \<rparr>) op')
    | _ \<Rightarrow> Code.abort (STR ''Operator in opt_dataflow_op breaks contract'') (\<lambda> _. \<oslash>))
-   (cfilter (\<lambda> op. is_busy sg op \<and> not_nop sg op)
+   (cfilter (\<lambda> op. not_nop sg op)
    (choices op))
    )"
+
+term show_myprod_frontier
+term show_loc
+
+term "fold (+)"
+
+definition "show_all_frontiers cimp = fold (+) (map (\<lambda> loc. STR ''Frontier: '' + show_loc loc +  STR '' = '' + show_myprod_frontier (frontier (cimp loc)) + STR ''; '') Enum.enum) (STR '''')"
+
+lemma opt_dataflow_op_code[code]:
+  "opt_dataflow_op sg op = Choice (cimage (\<lambda> op. case op of
+     Read (Inl nid) f \<Rightarrow> trace (STR ''Read frontier!'' + show_nat (to_nat_numeral nid)) (case propagate_all (summ sg) (pt_tr sg) of
+         Some conf' \<Rightarrow> let sg' = sg\<lparr> pt_tr := conf', upfro := (upfro sg)(nid := False) \<rparr> in
+         let imp_fron = (\<lambda> p. c_imp (pt_tr sg') (Loc nid (Trg p))) in trace (show_all_frontiers (c_imp (pt_tr sg'))) (Silent (opt_dataflow_op sg' (f (Inl (Inr (frontier o imp_fron))))))
+      | None \<Rightarrow> \<oslash>)
+   | Read (Inr (nid, p)) f \<Rightarrow>  (Read (nid, p) (\<lambda> x. opt_dataflow_op sg (f (Inr x))))
+   | Write op' (Inr (nid, p)) (Inr x) \<Rightarrow> trace (STR ''Write outside!'' + show_nat (to_nat_numeral nid)) (Write (opt_dataflow_op sg op') (nid, p) x)
+   | Silent op' \<Rightarrow> trace (STR ''Silent!'') (Silent (opt_dataflow_op sg op'))
+   | Write op' (Inl nid) (Inl (Inl st)) \<Rightarrow>
+     trace (STR ''Report progress!'' + show_nat (to_nat_numeral nid)) (Silent (opt_dataflow_op (sg\<lparr> upfro := (\<lambda> _. True), pt_tr :=change_multiplicities (summ sg) (extract_progress nid (nxt sg) st) (pt_tr sg) \<rparr>) op'))
+   | _ \<Rightarrow> Code.abort (STR ''Operator in opt_dataflow_op breaks contract'') (\<lambda> _. \<oslash>))
+   (cfilter (\<lambda> op. not_nop sg op)
+   (choices op))
+   )"
+  apply (simp only: delay_cset_def trace_simp id_def)
+  apply (subst opt_dataflow_op.code)
+  apply auto
+  done
+
+definition "opt_compile_dataflow chns dt = (let summary = antichain_from_list oo (dataflow_tree_to_graph dt) in
+                                    let op = dataflow_tree_to_operator chns dt in
+                                    let sg = init_subgraph summary in
+                                    opt_dataflow_op sg op)"
 
 
 end
