dataplane/Timely_Builder_Op.thy
@@ -24,12 +24,41 @@ corec builder_op where
       Inl (Inr f) \<Rightarrow> builder_op fb ips ops (os\<lparr>front := f, initia := True\<rparr>) logic
     | _ \<Rightarrow> Code.abort (STR ''Builder_op breaks contract'') (\<lambda>_. \<oslash>))
      else \<oslash>)
-    (Choice (cimage (\<lambda>p. Read (Some p) (\<lambda>x. case x of
+    ((Choice (cimage (\<lambda>p. Read (Some p) (\<lambda>x. case x of
       Inr (d, t) \<Rightarrow> builder_op fb ips ops (consumes os p t d) logic
-    | Inl _ \<Rightarrow> Code.abort (STR ''Builder_op breaks contract'') (\<lambda> _. \<oslash>))) ips))
+    | Inl _ \<Rightarrow> Code.abort (STR ''Builder_op breaks contract'') (\<lambda> _. \<oslash>))) ips)))
     (let (os', st) = obtain_progress os in send_progress (builder_op fb ips ops os' logic) st)
    )\<close>
 
+thm builder_op.code[of fb inps ops os logic]
+
+
+lemma
+  "builder_op fb inps ops os logic =
+Choice
+ ((\<lambda>b. case b of
+        None \<Rightarrow>
+          Choice
+           ((\<lambda>b. if b then if initia os then Choice ((\<lambda>os. Silent (builder_op fb inps ops os logic)) |`| logic os) else \<oslash>
+                  else Choice ((\<lambda>p. case outpu os p of x # xs \<Rightarrow> trace (STR ''Writing output'') (send_output (builder_op fb inps ops (os\<lparr>outpu := (outpu os)(p := xs)\<rparr>) logic) p x)) |`| cfilter (\<lambda>p. outpu os p \<noteq> []) ops)) |`|
+            {|True, False|})
+        | Some True \<Rightarrow>
+            Choice
+             ((\<lambda>b. if b
+                    then if fb
+                         then Read None
+                               (\<lambda>x. case x of Inl (Inl aa) \<Rightarrow> Code.abort STR ''Builder_op breaks contract'' (\<lambda>_. \<oslash>) | Inl (Inr f) \<Rightarrow> trace (STR ''Readingfrontier'') (builder_op fb inps ops (os\<lparr>front := f, initia := True\<rparr>) logic)
+                                     | Inr b \<Rightarrow> Code.abort STR ''Builder_op breaks contract'' (\<lambda>_. \<oslash>))
+                         else \<oslash>
+                    else Choice
+                          ((\<lambda>p. Read (Some p) (\<lambda>x. case x of Inl x \<Rightarrow> Code.abort STR ''Builder_op breaks contract'' (\<lambda>_. \<oslash>) | Inr (d, t) \<Rightarrow> builder_op fb inps ops (trace (STR ''Reading data'') (consumes os p t d)) logic)) |`| inps)) |`|
+              {|True, False|})
+        | Some False \<Rightarrow> let (os', st) = obtain_progress os in trace (STR ''Reporting progress'') (send_progress (builder_op fb inps ops os' logic) st)) |`|
+  {|None, Some True, Some False|})"
+  unfolding trace_simp
+  apply (subst builder_op.code)
+  apply simp
+  done
 
 subsection \<open>Rules for @{const builder_op}\<close>
 
